updating

coq/ChoiceAxiom.v
@@ -3,7 +3,21 @@ From Coq Require Import String.
 
 Import ListNotations.
 
-(* TODO: define as an axiom? *)
+(* TODO: remove? *)
 Lemma choice_axiom : forall (syms : list string), exists sym, ~ In sym syms.
+Proof.
+Admitted.
+
+Definition fresh_name (l : list string) : string.
+Admitted.
+
+Definition extend_names (l : list string) : list string.
+Admitted.
+
+Lemma fresh_name_lemma : forall l, ~ In (fresh_name l) l.
+Proof.
+Admitted.
+
+Lemma extend_names_lemma : forall l, extend_names l = (fresh_name l) :: l.
 Proof.
 Admitted.
